

# THEORY

$$X_m | \mu, \gamma \sim N\left(\mu, \frac{1}{\gamma}\right) \quad (\mu, \gamma) \sim NG(\mu_0, \lambda, \alpha, \beta)$$

$$\text{AS BEFORE, } P(\theta | D) = \frac{P(D | \theta) P(\theta)}{P(D)} \propto P(D | \theta) P(\theta)$$

$$\textcircled{1} P(D | \theta) \stackrel{\text{IID}}{=} \prod_{i=1}^N f_{\theta}(x_i) = \prod_{i=1}^N \sqrt{\frac{\gamma}{2\pi}} e^{-\frac{\gamma}{2}(x_i - \mu)^2}$$

$$\textcircled{2} P(\theta) = P(\mu, \gamma) = P(\gamma) P(\mu | \gamma) \stackrel{\text{prior}}{=} \frac{\beta^\alpha}{\Gamma(\alpha)} \gamma^{\alpha-1} e^{-\beta\gamma} \sqrt{\frac{\lambda\gamma}{2\pi}} e^{-\frac{\lambda\gamma}{2}(\mu - \mu_0)^2}$$

$$\stackrel{\text{BY THEORY}}{\propto} \gamma^{\alpha-\frac{1}{2}} e^{-\frac{\lambda\gamma}{2}[2\beta + (\mu - \mu_0)^2]}$$

$$\log(P(\mu, \gamma | X)) = \log\left(\prod_{n=1}^N P(x_n | \theta) P(\theta)\right) = \sum_{n=1}^N \log(P(x_n | \theta)) + \log P(\mu, \gamma)$$

$$\stackrel{\text{THEORY (PREVIOUSLY INTRODUCED)}}{=} \sum_{n=1}^N \log\left(\sqrt{\frac{\gamma}{2\pi}} e^{-\frac{\gamma}{2}(x_n - \mu)^2}\right) + \log\left(\frac{\beta^\alpha}{\Gamma(\alpha)\sqrt{2\pi}} \gamma^{\alpha-\frac{1}{2}} e^{-\beta\gamma} e^{-\frac{\lambda\gamma}{2}(\mu - \mu_0)^2}\right)$$

$$\propto_{\mu, \gamma} \sum_{n=1}^N \left[ \frac{1}{2} \log \gamma - \frac{\gamma}{2} (x_n - \mu)^2 \right] + \left( \alpha - \frac{1}{2} \right) \log \gamma - \beta \gamma - \frac{\lambda\gamma}{2} (\mu - \mu_0)^2$$

$$= \frac{N}{2} \log \gamma - \frac{\gamma}{2} \sum_{n=1}^N (x_n^2 + \mu^2 - 2\mu x_n) + \left( \alpha - \frac{1}{2} \right) \log \gamma - \beta \gamma - \frac{\lambda\gamma}{2} (\mu^2 + \mu_0^2 - 2\mu \mu_0)$$

$$= \left( \frac{N}{2} + \alpha - \frac{1}{2} \right) \log \gamma - \beta \gamma - \frac{\gamma}{2} \left[ \mu^2 (N + \lambda) - 2\mu \left( \sum_{n=1}^N x_n + \mu_0 \lambda \right) + \sum_{n=1}^N x_n^2 + \lambda \mu_0^2 \right]$$

$$= \left( \frac{N}{2} + \alpha - \frac{1}{2} \right) \log \gamma - \beta \gamma - \frac{\gamma}{2} (N + \lambda) \left[ \mu^2 - \frac{2\mu}{N + \lambda} \left( \sum_{n=1}^N x_n + \mu_0 \lambda \right) + \frac{1}{N + \lambda} \left( \sum_{n=1}^N x_n^2 + \lambda \mu_0^2 \right) \right]$$

$$= \left( \frac{N}{2} + \alpha - \frac{1}{2} \right) \log \gamma - \beta \gamma - \frac{\gamma}{2} (N + \lambda) \left[ \mu^2 - \frac{2\mu}{N + \lambda} \left( \sum_{n=1}^N x_n + \mu_0 \lambda \right) + C \right]$$

$$= \left( \frac{N}{2} + \alpha - \frac{1}{2} \right) \log \gamma - \gamma \left( \beta + \frac{C}{2} (N + \lambda) \right) - \frac{\gamma}{2} (N + \lambda) \left[ \mu^2 - 2\mu \frac{1}{N + \lambda} \left( \sum_{n=1}^N x_n + \mu_0 \lambda \right) + \frac{\gamma}{2} (N + \lambda) D^2 - \frac{\gamma}{2} (N + \lambda) D^2 \right]$$

GOAL:  
COMPLETE THE SQUARES

$$= \underbrace{\left( \frac{N}{2} + \alpha - \frac{1}{2} \right)}_{\alpha^*} \log \gamma - \underbrace{\gamma \left( \beta + \frac{N + \lambda}{2} C \right)}_{\beta^*} - \underbrace{\frac{\gamma}{2} (N + \lambda)}_{\lambda^*} \left[ \mu^2 - 2\mu \underbrace{D}_{\mu_0^*} + \underbrace{D^2}_{\mu_0^{*2}} \right]$$

$$= \left( \alpha^* - \frac{1}{2} \right) \log \gamma - \beta^* \gamma - \frac{\gamma}{2} \lambda^* (\mu - \mu_0^*)^2$$

$$= \text{NORMAL GAUSSIAN}(\mu_0^*, \lambda^*, \alpha^*, \beta^*)$$

## PARAMETERS:

$$\alpha^* = \frac{N}{2} + \alpha$$

$$\lambda^* = N + \lambda$$

$$\mu^* = D = \frac{1}{N + \lambda} \left( \sum_{n=1}^N x_n + \mu_0 \lambda \right) = \frac{1}{\lambda^*} \left( \sum_{n=1}^N x_n + \mu_0 \lambda \right)$$

$$\text{RECALL } C = \frac{1}{N + \lambda} \left( \sum_{n=1}^N x_n^2 + \lambda \mu_0^2 \right)$$

$$\begin{aligned} \beta^* &= \beta + \frac{N + \lambda}{2} (C - D^2) = \beta + \frac{\lambda^*}{2} \left( \frac{1}{\lambda^*} \left( \sum_{n=1}^N x_n^2 + \lambda \mu_0^2 \right) - \mu_0^{*2} \right) \\ &= \beta + \frac{1}{2} \left( \sum_{n=1}^N x_n^2 + \lambda \mu_0^2 - \lambda^* \mu_0^{*2} \right) \end{aligned}$$